modified general theorem in Loading.v proved closed forward simulation from cc_compcert

driver/CompilerClosed.v
@@ -71,7 +71,11 @@ Inductive final_asm : int -> reply li_asm -> Prop :=
      (* rs # PC = Vnullptr -> *)
      rs # RAX = Vint r ->
     final_asm r (rs,m).
-    
+
+Inductive valid_world_cc_compcert : ccworld cc_compcert -> Prop :=
+|valid_w_intro: forall se j1 j2 m1 m2 m3 Hm1 Hm2 rs,
+    valid_world_cc_compcert (se, row se m1,(se,(se,main_sg),(se,cajw (injpw j1 m1 m2 Hm1) main_sg rs,injpw j2 m2 m3 Hm2))).
+
 Section Initial.
   
   Variable m0 : mem.
@@ -128,6 +132,9 @@ Section Initial.
   split. split. exact se. exact init_w_cainjp. exact init_w_injp.
   Defined.  
 
+  Theorem valid_init_w : valid_world_cc_compcert init_w.
+  Proof. constructor. Qed.
+    
   Theorem sound_ro : sound_memory_ro se m0.
   Proof.
     eapply initial_ro_sound; eauto.
@@ -191,7 +198,7 @@ Lemma match_initial_forward_ca : forall q1,
     initial_c q1 -> exists wB q2,
       match_query cc_compcert wB q1 q2 /\
         match_senv cc_compcert wB se tse /\
-        initial_asm q2.
+        initial_asm q2 /\ valid_world_cc_compcert wB.
 Proof.
   intros. inv H. rename m into m0.
   caseEq (Mem.alloc m0 0 0). intros m bsp Hdummy.
@@ -238,26 +245,23 @@ Proof.
   - (*init_asm*)
     econstructor; eauto. rewrite skel_eq; eauto.
     rewrite main_id_eq, symtbl_eq; eauto. reflexivity.
+  - constructor.
 Qed.
 
 Lemma match_final_forward_ca : forall r r1 r2 wB,
-    match_reply cc_compcert wB r1 r2 ->
+    match_reply cc_compcert wB r1 r2 -> valid_world_cc_compcert wB ->
     final_c r r1 -> final_asm r r2.
 Proof.
   intros. inv H0.
-  destruct wB as ([a [b1 b2]] & [c [d1 d2]] & [e f] & g).
-  destruct H as [r1 [Hr1 [r2' [Hr2 [r3 [Hr3 Hr4]]]]]].
-  inv Hr1. inv Hr2. inv Hr3. inv Hr4. inv H. simpl in H0.
-  destruct H1.
-  red in H. inv H.
+  destruct H as [r1' [Hr1 [r2' [Hr2 [r3 [Hr3 Hr4]]]]]].
+  inv Hr1. inv Hr2. inv Hr3. inv Hr4. inv H. simpl in H0. inv H1.
+  destruct H2. inv H.
   destruct r2. inv H1.
   constructor. unfold Conventions1.loc_result in tres. subst tres.
-  replace (Archi.ptr64) with true in H3 by reflexivity.
-  unfold Conventions1.loc_result_64 in H3.
-  assert (sg = main_sg). admit.
-  rewrite H1 in H3. simpl in H3. simpl in H.
-  inv H3. specialize (H RAX). rewrite <- H20 in H. inv H. reflexivity.
-Admitted.
+  replace (Archi.ptr64) with true in H7 by reflexivity.
+  unfold Conventions1.loc_result_64 in H7. simpl in H7.
+  inv H7. specialize (H RAX). rewrite <- H5 in H. inv H. reflexivity.
+Qed.
 
 Definition close_c := close_semantics L_c initial_c final_c.
 Definition close_asm := close_semantics L_asm initial_asm final_asm.
@@ -272,390 +276,8 @@ Qed.
   
 End CLOSE_FORWARD.
 
-(* Checking whether the defs and lemmas from are typed as we want in the outside of the Section.
+(* Checking whether the defs and lemmas from are typed as we want in the outside of the Section. *)
 Check close_c.
 Check close_asm.
 Check closed_forward_simulation_cc_compcert.
-*)
-  
-(*
-Section CLOSE_COMPCERT.
-Import Closed.
 
-Variable p : Csyntax.program.
-Variable tp : Asm.program.
-Hypothesis transf : transf_c_program p = OK tp.
-Let se := Genv.symboltbl (erase_program p).
-
-Variable main_block_c : block.
-Variable m0_c : mem.
-
-Let liA1 := li_c.
-Let liB1 := li_c.
-Let sg := AST.mksignature nil (AST.Tret AST.Tint) AST.cc_default.
-Let main_function_value_c := Vptr main_block_c Ptrofs.zero.
-Let query1 := cq main_function_value_c sg nil m0_c.
-
-Inductive reply1 : int -> c_reply -> Prop :=
-  | reply1_intro: forall r m,
-      reply1 r (cr (Vint r) m).
-
-Let s1 := Csem.semantics p.
-Let se1 := se.
-Let lts1' := (Smallstep.activate s1 se1).
-
-Let ge_c' := Smallstep.globalenv (s1 se).
-Let ge_c := Csem.genv_genv ge_c'.
-Variable main_c : Csyntax.fundef.
-Hypothesis Hinitial_state_c :
-  Genv.init_mem (erase_program p) = Some m0_c /\
-  Genv.find_symbol se p.(prog_main) = Some main_block_c /\
-  Genv.find_funct_ptr ge_c main_block_c = Some main_c.
-
-Import Asm.
-
-Let s2 := Asm.semantics tp.
-Let ge_asm := Smallstep.globalenv (s2 se).
-Variable m0_asm' m0_asm : mem.
-Variable dsp : block. (** The dummy block as stack pointer *)
-Hypothesis Hinitial_state_asm1: Genv.init_mem (erase_program tp) = Some m0_asm'.
-Hypothesis Hinitial_state_asm2: Mem.alloc m0_asm' 0 0 = (m0_asm, dsp).
-
-Let liA2 := li_asm.
-Let liB2 := li_asm.
-Let rs0 :=
-    (Pregmap.init Vundef)
-    # PC <- (Genv.symbol_address ge_asm tp.(prog_main) Ptrofs.zero)
-    # RA <- Vnullptr
-    # RSP <- (Vptr dsp Ptrofs.zero).
-
-Let query2 := (rs0, m0_asm).
-
-Inductive reply2: int -> (regset * mem) -> Prop :=
-  | reply2_intro: forall r (rs:regset) m,
-      (* rs#PC = Vnullptr -> *)
-      rs#RAX = Vint r ->
-      reply2 r (rs, m).
-Let se2 := se.
-Let lts2' := (Smallstep.activate s2 se2).
-
-Lemma erase_same: erase_program p = erase_program tp.
-Proof.
-  exploit transf_c_program_match; eauto. intro MATCH.
-  unfold match_c_prog in MATCH. simpl in MATCH. repeat destruct MATCH as (? & MATCH).
-  fold Csyntax.fundef. remember p as xx.
-  rename xx into p', p into xx. rename p' into p.
-  match goal with
-  | H: ?P p ?p2 |- _ => rewrite Heqxx in H
-  end.
-  rewrite Heqxx. clear Heqxx.
-  Ltac mp H p1 p2 :=
-    unfold Linking.match_program in H;
-    match type of H with
-    | Linking.match_program_gen _ _ _ _ _ =>
-        apply Linking.match_program_skel in H;
-        try fold CminorSel.fundef in H;
-        try fold RTL.fundef in H;
-        rewrite H; clear H p1;
-        rename p2 into p1
-    | Linking.match_program_gen _ _ _ _ _ /\ _ =>
-        let H' := fresh "H" in
-        let garbage := fresh "H" in
-        destruct H as (H' & garbage);
-        clear garbage;
-        mp H' p1 p2
-    end.
-  Ltac try_rewrite xx := match goal with
-  | H: ?P xx ?p2 |- _ =>
-    unfold P in H; mp H xx p2
-  | H: match_if ?cond ?P xx ?p2 |- _ =>
-    unfold match_if, P in H;
-    let H' := fresh "H" in
-    assert (H' : erase_program xx = erase_program p2) by (destr_in H; mp H xx p2; auto);
-    rewrite H';
-    clear H' H xx;
-    rename p2 into xx
-  end.
-  repeat try_rewrite xx.
-  unfold Unusedglobproof.match_prog in H12.
-  destruct H12 as (u & VALID & MATCH').
-  inv MATCH'. rewrite <- match_prog_skel.
-  clear match_prog_main match_prog_public match_prog_def match_prog_skel VALID xx u.
-  rename x12 into xx.
-  repeat try_rewrite xx.
-  auto.
-Qed.
-
-Lemma m0_same: m0_c = m0_asm'.
-Proof.
-  rewrite erase_same, Hinitial_state_asm1 in Hinitial_state_c.
-  destruct Hinitial_state_c. inv H. auto.
-Qed.
-
-Let ccA : callconv liA1 liA2 := cc_compcert.
-Let ccB : callconv liB1 liB2 := cc_compcert.
-
-Lemma Hvalid: Genv.valid_for (erase_program p) se1.
-Proof.
-  red. intros. rewrite Genv.find_info_symbol in H. destruct H as (b & []).
-  exists b, g. unfold se1, se. split; auto. split; auto.
-  destruct g; constructor. constructor.
-  destruct v. constructor; constructor.
-Qed.
-
-Lemma m0_inject_c: Mem.inject (Mem.flat_inj (Mem.support m0_c)) m0_c m0_c.
-Proof.
-  apply (Genv.initmem_inject (erase_program p)).
-  apply Hinitial_state_c.
-Qed.
-
-Lemma m0_inject_c_asm: Mem.inject (Mem.flat_inj (Mem.support m0_c)) m0_c m0_asm.
-Proof.
-  eapply Mem.alloc_right_inject.
-  2: apply Hinitial_state_asm2; eauto.
-  rewrite <- m0_same.   apply m0_inject_c.
-Qed.
-
-Let j' := fun b => if eq_block b dsp then Some (dsp ,0) else (Mem.flat_inj (Mem.support m0_c)) b.
-
-Lemma m0_inject_asm : Mem.inject j' m0_asm m0_asm.
-Proof.
-  generalize m0_inject_c. intro H. rewrite m0_same in H.  
-  exploit Mem.alloc_parallel_inject. eauto.
-  apply Hinitial_state_asm2. reflexivity. reflexivity.
-  intros (j'1 & m2' & dsp' & A &B & C & D& E).
-  generalize Hinitial_state_asm2. intro H2. rewrite A in H2. inv H2.
-  replace j' with j'1. eauto.
-  apply Axioms.functional_extensionality.
-  intros. unfold j'. destr. subst. eauto. rewrite m0_same. eapply E; eauto.
-Qed.
-
-Let wB : ccworld ccB.
-  unfold ccB, cc_compcert, CA.cc_c_asm_injp. simpl.
-  (* ro *)
-  split. split. exact se. split. exact se. exact m0_c.
-  (* wt_c *)
-  split. split. exact se. split. exact se. exact sg.
-  (* cc_c_asm_injp *)
-  split. split. exact se. split.
-  simpl. econstructor. exact m0_inject_c_asm. exact sg. exact rs0.
-  (* cc_asm injp *)
-  econstructor. exact m0_inject_asm.
-Defined.
-
-Hypothesis closed:
-  forall v id sg, Genv.find_funct (Genv.globalenv se tp) v <> Some (External (EF_external id sg)).
-
-Lemma closed2 : forall s q, Smallstep.safe lts2' s -> ~ Smallstep.at_external lts2' s q.
-Proof.
-  unfold lts2', s2, se2, semantics. simpl. intros. intro.
-  destruct s. inv H0.
-  eapply closed; eauto.
-Qed.
-
-Lemma reply_sound2: forall s r, Smallstep.final_state lts2' s r -> exists i, reply2 i r.
-Proof.
-  unfold lts2', s2, se2. simpl. intros. destruct s.
-  inversion H. eexists. econstructor.
-  admit.
-Abort.
-(*
-1. rs#RAX should be a integer
-2. rs#PC should be Vnullptr
-
- *)
-
-Lemma sound_memory_ro: ValueAnalysis.sound_memory_ro se m0_c.
-Proof.
-  unfold se. destruct Hinitial_state_c. clear H0.
-  eapply ValueAnalysis.initial_ro_sound; eauto.
-Qed.
-
-Lemma main_block_genv: Genv.find_symbol se (prog_main tp) = Some main_block_c.
-Proof.
-  destruct Hinitial_state_c as [? []].
-  pose proof erase_same. inv H2. simpl in H0. rewrite H0. auto.
-Qed.
-
-Lemma has_main_block: sup_In main_block_c (Mem.support m0_c).
-Proof.
-  destruct Hinitial_state_c as [? []].
-  eapply Genv.find_symbol_not_fresh; eauto.
-Qed.
-
-Lemma size_0: Conventions.size_arguments sg = 0.
-Proof.
-  unfold Conventions.size_arguments, Conventions1.loc_arguments. simpl.
-  destruct Archi.ptr64, Archi.win64; simpl; auto.
-Qed.
-
-Lemma Hmatch_query : match_query ccB wB query1 query2.
-Proof.
-  simpl.
-  exists query1. split.
-  constructor. constructor. exact sound_memory_ro.
-  exists query1. split.
-  constructor. split. reflexivity. simpl. auto.
-  exists query2. split.
-  unfold query1, query2. econstructor; simpl.
-  unfold Conventions1.loc_arguments. cbn.
-  destruct Archi.ptr64, Archi.win64; simpl; constructor.
-  unfold rs0. simpl.
-  unfold main_function_value_c, Genv.symbol_address.
-  rewrite main_block_genv.
-  econstructor. unfold Mem.flat_inj. pose proof has_main_block. destr.
-  rewrite Ptrofs.add_zero. auto.
-  intros. rewrite size_0 in H. inv H. extlia.
-  cbn. unfold Vnullptr, Tptr. destruct Archi.ptr64; simpl; auto.
-  cbn. unfold Vnullptr, Tptr. destruct Archi.ptr64; simpl; auto.
-  constructor. eapply Mem.valid_new_block. eapply Hinitial_state_asm2.
-  econstructor. apply size_0.
-  unfold main_function_value_c. discriminate.
-  discriminate.
-  unfold cc_asm_match'. simpl. split; [|split].
-  intros. unfold rs0.
-  destruct (PregEq.eq r RSP); [subst; rewrite Pregmap.gss|
-  rewrite Pregmap.gso; auto; destruct (PregEq.eq r RA); [subst; rewrite Pregmap.gss|
-  rewrite Pregmap.gso; auto; destruct (PregEq.eq r PC); [subst; rewrite Pregmap.gss|
-                                                          rewrite Pregmap.gso; auto]]].
-  econstructor; eauto. unfold j'. destr. rewrite Ptrofs.add_zero. reflexivity.
-  unfold Vnullptr. destr; constructor.
-  unfold Genv.symbol_address. destr; econstructor.
-  unfold ge_asm in Heqo. simpl in Heqo. rewrite main_block_genv in Heqo. inv Heqo.
-  unfold j'. unfold Mem.flat_inj. pose proof has_main_block. destr.
-  pose proof Hinitial_state_asm2. inv e.
-  apply Mem.fresh_block_alloc in H0. rewrite <- m0_same in H0. elim H0. rewrite <- H1. eauto.
-  destr.
-  rewrite Ptrofs.add_zero. auto.
-  unfold rs0.
-  rewrite Pregmap.gso; [|discriminate].
-  rewrite Pregmap.gso; [|discriminate].
-  rewrite Pregmap.gss.
-  unfold ge_asm. simpl. unfold Genv.symbol_address. rewrite main_block_genv. discriminate.
-  constructor.
-Qed.
-
-Lemma Hmatch_reply1 : forall r r1 r2,
-    match_reply ccB wB r1 r2 ->
-    reply1 r r1 -> reply2 r r2.
-Proof.
-  intros. destruct H as [r_c [Hro [r_c' [Hwt [r_a [Hca Hasm]]]]]].
-  inv H0. inv Hro. inv Hwt. inv Hca.
-  destruct Hasm as [wj [Hw Hr]].
-  destruct r2. inv Hr.
-  constructor.
-  (*r0 RAX -> rs' RAX -> Vint r via the signature sg*)
-  assert (tres = rs' RAX).
-  { unfold tres. unfold sg. unfold CA.rs_getpair.
-    unfold Conventions1.loc_result, Conventions1.loc_result_64, Conventions1.loc_result_32. simpl. destruct Archi.ptr64; reflexivity.
-  }
-  inv H8. generalize (H1 RAX).
-  intro. simpl in H4. rewrite <- H3 in H4. rewrite <- H6 in H4.
-  inv H4. reflexivity.
-Qed.
-
-Lemma Hmatch_reply2 : forall r r1 r2,
-    match_reply ccB wB r1 r2 ->
-    reply2 r r2 ->
-    reply1 r r1.
-Proof.
-  intros. destruct H as [r_c [Hro [r_c' [Hwt [r_a [Hca Hasm]]]]]].
-  inv H0. inv Hro. inv Hwt. inv Hca.
-  destruct Hasm as [wj [Hw Hr]].
-  unfold Conventions1.loc_result, Conventions1.loc_result_64, Conventions1.loc_result_32 in tres. unfold sg in tres.
-  assert (Archi.ptr64 = true). admit.
-  unfold CA.rs_getpair in tres. simpl in tres.
-  unfold map_rpair in tres. simpl in tres.
-  assert (tres = rs' RAX).
-  unfold tres. rewrite H2. simpl. reflexivity.
-  rewrite H3 in H7.
-  admit. (*problem: res can be Vundef*)
-Abort.
-
-Lemma Hmatch_reply : forall r r1 r2,
-  match_reply ccB wB r1 r2 ->
-  reply1 r r1 <-> reply2 r r2.
-Proof.
-Abort.
-
-Lemma m0_se_support : Genv.genv_sup se = Mem.support m0_c.
-Proof.
-  unfold se. rewrite erase_same. rewrite m0_same.
-  eapply Genv.init_mem_genv_sup; eauto.
-Qed.
-
-Lemma match_se_initial : Genv.match_stbls (Mem.flat_inj (Mem.support m0_c)) se se.
-Proof.
-  pose proof m0_se_support as SUP.
-  constructor; intros; eauto.
-  - rewrite <- SUP. unfold Mem.flat_inj. rewrite pred_dec_true; eauto.
-  - rewrite <- SUP. exists b2. unfold Mem.flat_inj. rewrite pred_dec_true; eauto.
-  - unfold Mem.flat_inj in H. destruct Mem.sup_dec in H; inv H. reflexivity.
-  - unfold Mem.flat_inj in H. destruct Mem.sup_dec in H; inv H. reflexivity.
-  - unfold Mem.flat_inj in H. destruct Mem.sup_dec in H; inv H. reflexivity.
-Qed.
-    
-Lemma Hmatch_senv : match_senv ccB wB se1 se2.
-Proof.
-  pose proof m0_se_support as SUP.
-  pose proof Hinitial_state_asm2 as ALLOC.
-  apply Mem.fresh_block_alloc in ALLOC as FRESH; eauto.
-  rewrite <- m0_same in FRESH.
-  assert (SUPINCL: Mem.sup_include (Mem.support m0_c) (Mem.support m0_asm)).
-  apply Mem.support_alloc in ALLOC. rewrite ALLOC. red.
-  intros. apply Mem.sup_incr_in2; eauto. rewrite <- m0_same. eauto.
-  unfold ccB, cc_compcert, se1, se2. simpl.
-  split; [|split; [|split]].
-  constructor. auto.
-  constructor. auto.
-  constructor. apply match_se_initial; eauto.
-  rewrite SUP. eauto.
-  rewrite SUP. eauto.
-  constructor.
-  eapply Genv.match_stbls_incr. apply match_se_initial.
-  red. intros. unfold j'. destr. subst b. unfold Mem.flat_inj in H. destr_in H.
-  intros. unfold j' in H0. destr_in H0. subst b1. inv H0.
-  rewrite SUP. split; eauto.
-  rewrite SUP. eauto.
-  rewrite SUP. eauto.
-Qed.
-
-(* Lemma open_fsim : Smallstep.forward_simulation ccA ccB s1 s2.
-Proof.
-  exploit clight_semantic_preservation.
-  apply transf_c_program_match. auto. *)
-
-Lemma open_simulation: Smallstep.backward_simulation ccA ccB s1 s2.
-Proof.
-  apply c_semantic_preservation, transf_c_program_match. auto.
-Qed.
-
-(*
-Lemma compcert_close_sound :
-  backward_simulation (L1 query1 reply1 s1 se1) (L2 query2 reply2 s2 se2).
-Proof.
-  eapply close_sound_backward; eauto using
-    closed2, reply_sound2, Hvalid, Hmatch_query, Hmatch_senv, open_simulation.
-  intros. eapply Hmatch_reply2; eauto.
-Qed.
- *)
-
-Lemma compcert_close_sound_forward : 
-  forward_simulation (L1 query1 reply1 s1 se2) (L2 query2 reply2 s2 se2).
-Proof.
-  eapply close_sound_forward; eauto.
-  exact Hvalid. eapply Hmatch_query; eauto. exact Hmatch_senv.
-  intros.
-  eapply Hmatch_reply1; eauto.
-  admit. (*The missing Open Sim *)
-Admitted.
-End CLOSE_COMPCERT.
-*)
-
-
-(*
-Lemma loading_forward: forall L1 L2,
-    Smallstep.forward_simulation cc_compcert cc_compcert L1 L2 ->
-    exists CL1 CL2,
-    forward_simulation CL1 CL2.
-*)
